Finish proving triples for ExMach memory ops; switch StatDB to use ExMach as base layer.

src/Examples/ExMach/WeakestPre.v
@@ -12,7 +12,7 @@ Set Default Proof Using "Type".
 Class exmachG Σ := ExMachG {
                      exm_invG : invG Σ;
                      exm_mem_inG :> seq_heapG nat nat Σ;
-                     exm_disk_inG :> seq_heapG nat nat Σ;
+                     exm_disk_inG :> gen_heapG nat nat Σ;
                      exm_current : nat;
                    }.
 
@@ -23,18 +23,15 @@ Instance exmachG_irisG `{exmachG Σ} : irisG ExMach.Op ExMach.l Σ :=
     iris_invG := exm_invG;
     state_interp :=
       (λ s, ∃ mems disks, @seq_heap_ctx _ _ _ _ _ (exm_mem_inG) mems ∗
-                          @seq_heap_ctx _ _ _ _ _ (exm_disk_inG) disks ∗
+                          gen_heap_ctx disks ∗
                             ⌜ mems (exm_current) = mem_state s ∧
-                              disks (exm_current) = disk_state s ∧
+                              disks = disk_state s ∧
                               (∀ k, k > exm_current → mems k = mem_state (crash_fun s)) ∧
-                              (∀ k, k > exm_current → disks k = disk_state (crash_fun s)) ∧
                               (∀ i, is_Some (mem_state s !! i) → i < size) ∧
                               (∀ i, is_Some (disk_state s !! i) → i < size) ⌝
       )%I
   }.
 
-Section lifting.
-Context `{exmachG Σ}.
 
 Definition mem_mapsto_vs k v k' :=
   match Nat.compare k' k with
@@ -43,20 +40,22 @@ Definition mem_mapsto_vs k v k' :=
   | Gt => Some 0
   end.
   
-Check mapsto_fun.
-Local Notation "l ↦{ q } v @N" :=
+Global Notation "l ↦{ q } v @N" :=
   (@mapsto_fun _ _ _ _ _ (exm_mem_inG) l q (mem_mapsto_vs (exm_current) v))
   (at level 20, q at level 50, format "l  ↦{ q } v @N") : bi_scope.
-Local Notation "l ↦ v @N " :=
+Global Notation "l ↦ v @N " :=
   (@mapsto_fun _ _ _ _ _ (exm_mem_inG) l 1 (mem_mapsto_vs (exm_current) v))
   (at level 20) : bi_scope.
 
-Local Notation "l ↦{ q } v @C" :=
+Global Notation "l ↦{ q } v @C" :=
   (@mapsto_fun _ _ _ _ _ (exm_mem_inG) l q (mem_mapsto_vs (S exm_current) v))
   (at level 20, q at level 50, format "l  ↦{ q } v @C") : bi_scope.
-Local Notation "l ↦ v @C" :=
+Global Notation "l ↦ v @C" :=
   (@mapsto_fun _ _ _ _ _ (exm_mem_inG) l 1 (mem_mapsto_vs (S exm_current) v))
   (at level 20) : bi_scope.
+
+Section lifting.
+Context `{exmachG Σ}.
 
 Lemma nat_compare_lt_Lt: ∀ n m : nat, n < m → (n ?= m) = Lt.
 Proof. intros. by apply nat_compare_lt. Qed.
@@ -72,7 +71,7 @@ Proof.
   iIntros (e2 σ2 Hstep) "!>".
   inversion Hstep; subst.
   iDestruct "Hown" as (mems disks) "(Hown1&Hown2&Hp)".
-  iDestruct "Hp" as %(Heq_mem&?&Hcrash_mem&Hcrash_disks&Hsize&?).
+  iDestruct "Hp" as %(Heq_mem&?&Hcrash_mem&Hsize&?).
   iDestruct (seq_heap_valid with "Hown1 Hi") as %Hin_bound.
   iMod (@seq_heap_update _ _ _ _ _ exm_mem_inG mems i
                          (mem_mapsto_vs (exm_current) v')
@@ -96,7 +95,6 @@ Proof.
       apply init_zero_insert_zero. apply Hsize.
       exists v'. rewrite -Heq_mem. apply Hin_bound.
       rewrite /mem_mapsto_vs Nat.compare_refl //=.
-    * done.
     * rewrite /set_mem/set_default//= => i'.
       specialize (Hsize i').
       destruct ((mem_state σ) !! i) eqn:Heq; rewrite Heq.
@@ -117,7 +115,7 @@ Proof.
   iIntros (e2 σ2 Hstep) "!>".
   inversion Hstep; subst.
   iDestruct "Hown" as (mems disks) "(Hown1&Hown2&Hp)".
-  iDestruct "Hp" as %(Heq_mem&?&Hcrash_mem&Hcrash_disks&Hsize&?).
+  iDestruct "Hp" as %(Heq_mem&?&Hcrash_mem&Hsize&?).
   iDestruct (seq_heap_valid with "Hown1 Hi") as %Hin_bound.
   iModIntro. iSplitR "Hi HΦ".
   - iExists _, _. iFrame; iPureIntro; split_and!; eauto.
@@ -130,11 +128,18 @@ Qed.
 
 Lemma mem_crash i v : i ↦ v @N -∗ i ↦ 0 @C.
 Proof.
-  rewrite /
-  iIntros.
+  eapply mapsto_fun_weaken with (k := exm_current).
+  intros k. rewrite /mem_mapsto_vs. destruct nat_eq_dec; subst.
+  - rewrite nat_compare_lt_Lt; auto.
+  - destruct (Nat.compare_spec k (exm_current)).
+    * rewrite nat_compare_lt_Lt; try congruence.
+    * rewrite nat_compare_lt_Lt; try congruence; lia.
+    * destruct (Nat.compare_spec k (S exm_current)); auto.
+      lia.
+Qed.
 
 Lemma cas_non_stuck i v1 v2 σ:
-  ¬ Var.l.(step) (CAS i v1 v2) σ Err.
+  ¬ ExMach.l.(step) (CAS i v1 v2) σ Err.
 Proof.
   intros Hstuck. destruct Hstuck as [Hread|(v'&?&Hread&Hrest)].
   - inversion Hread.
@@ -143,39 +148,81 @@ Qed.
 
 Lemma wp_cas_fail s E i v1 v2 v3 :
   v1 ≠ v2 →
-  {{{ ▷ i ↦ v1 }}} cas i v2 v3 @ s; E {{{ RET v1; i ↦ v1 }}}.
+  {{{ ▷ i ↦ v1 @N }}} cas i v2 v3 @ s; E {{{ RET v1; i ↦ v1 @N }}}.
 Proof.
   iIntros (Hneq Φ) ">Hi HΦ". iApply wp_lift_call_step.
-  iIntros (σ) "Hown". destruct_state σ "Hown".
+  iIntros (σ) "Hown".
   iModIntro. iSplit.
   { destruct s; auto using cas_non_stuck. }
   iIntros (e2 σ2 Hstep) "!>".
+  iDestruct "Hown" as (mems disks) "(Hown1&Hown2&Hp)".
+  iDestruct "Hp" as %(Heq_mem&?&Hcrash_mem&Hsize&?).
+  iDestruct (seq_heap_valid with "Hown1 Hi") as %Hin_bound.
+  assert (Hlookup: σ.(mem_state) !! i = Some v1).
+  { rewrite -Heq_mem. apply Hin_bound.
+    rewrite /mem_mapsto_vs Nat.compare_refl //=. }
   inversion Hstep as (v'&σ2'&Hread&Hrest); subst.
+  rewrite /get_mem/get_default/reads Hlookup in Hread.
   inversion Hread; subst.
-  destruct i; iDestruct (reg_agree with "Hi [$]") as "%"; subst;
-    iFrame; simpl;
-  (destruct (nat_eq_dec); [ by (subst; exfalso; eauto)|];
-  inversion Hrest; subst;
-  iFrame; by iApply "HΦ").
+  destruct nat_eq_dec; first by exfalso.
+  inversion Hrest; subst.
+  iModIntro. iSplitR "Hi HΦ".
+  - iExists _, _. iFrame; iPureIntro; split_and!; eauto.
+  - by iApply "HΦ".
 Qed.
 
 Lemma wp_cas_suc s E i v1 v2 :
-  {{{ ▷ i ↦ v1 }}} cas i v1 v2 @ s; E {{{ RET v1; i ↦ v2 }}}.
+  {{{ ▷ i ↦ v1 @N }}} cas i v1 v2 @ s; E {{{ RET v1; i ↦ v2 @N }}}.
 Proof.
   iIntros (Φ) ">Hi HΦ". iApply wp_lift_call_step.
-  iIntros (σ) "Hown". destruct_state σ "Hown".
+  iIntros (σ) "Hown".
   iModIntro. iSplit.
   { destruct s; auto using cas_non_stuck. }
-  iIntros (e2 σ2 Hstep) "!>".
+  iIntros (v2' σ2 Hstep) "!>".
+  iDestruct "Hown" as (mems disks) "(Hown1&Hown2&Hp)".
+  iDestruct "Hp" as %(Heq_mem&?&Hcrash_mem&Hsize&?).
+  iDestruct (seq_heap_valid with "Hown1 Hi") as %Hin_bound.
+  assert (Hlookup: σ.(mem_state) !! i = Some v1).
+  { rewrite -Heq_mem. apply Hin_bound.
+    rewrite /mem_mapsto_vs Nat.compare_refl //=. }
   inversion Hstep as (v'&σ2'&Hread&Hrest); subst.
   inversion Hread; subst.
-  destruct i; iDestruct (reg_agree with "Hi [$]") as "%"; subst;
-  (destruct (nat_eq_dec); [| simpl in *; congruence]);
-  inversion Hrest as ([]&?&Hputs&Hpure); inversion Hputs; inversion Hpure; subst;
-     iMod (reg_update _ v2 with "Hi [$]") as "(Hi&$)"; subst;
-    iFrame; simpl;
-  inversion Hrest; subst;
-  iFrame; by iApply "HΦ".
+  rewrite /get_mem/get_default/reads Hlookup in Hread Hrest.
+  destruct nat_eq_dec; last by eauto.
+  destruct Hrest as ([]&?&Hputs&Hpure).
+  inversion Hpure; subst.
+  inversion Hputs; inversion Hpure; subst.
+  iMod (@seq_heap_update _ _ _ _ _ exm_mem_inG mems i
+                         (mem_mapsto_vs (exm_current) _)
+                         (mem_mapsto_vs (exm_current) v2)
+          with "Hown1 Hi") as "(Hown1&Hi)".
+  { intros k. rewrite /mem_mapsto_vs.  destruct Nat.compare => //=. clear; firstorder. }
+  iModIntro.
+  iSplitR "Hi HΦ".
+  - iExists _, _. iFrame.
+    iPureIntro. split_and!.
+    * rewrite /mem_mapsto_vs Nat.compare_refl.
+      rewrite /set_mem/set_default//=. rewrite -Heq_mem.
+      specialize (Hin_bound exm_current v2').
+      rewrite Hin_bound //.
+      rewrite /mem_mapsto_vs Nat.compare_refl //=.
+    * done.
+    * intros k Hgt.
+      rewrite /mem_mapsto_vs. rewrite nat_compare_gt_Gt /=; last auto.
+      rewrite /crash_fun/set_mem. rewrite /= Hcrash_mem; last auto.
+      rewrite /crash_fun/set_mem/=.
+      apply init_zero_insert_zero. apply Hsize.
+      exists v2'. rewrite -Heq_mem. apply Hin_bound.
+      rewrite /mem_mapsto_vs Nat.compare_refl //=.
+    * rewrite /set_mem/set_default//= => i'.
+      specialize (Hsize i').
+      destruct ((mem_state σ2') !! i) eqn:Heq; rewrite Heq.
+      ** case (decide (i = i')).
+         *** intros -> ?. apply Hsize; eauto.
+         *** intros ?. rewrite lookup_insert_ne //=.
+      ** apply Hsize.
+    * eauto.
+  - iApply "HΦ". eauto.
 Qed.
 
 End lifting.
@@ -190,34 +237,34 @@ Instance subG_lockΣ {Σ} : subG lockΣ Σ → lockG Σ.
 Proof. solve_inG. Qed.
 
 Section lock.
-  Context `{!varG Σ, !lockG Σ}.
+  Context `{!exmachG Σ, !lockG Σ}.
 
-  Definition lock_inv (γ : gname) (P : iProp Σ) : iProp Σ :=
-    ((Lock ↦ 0 ∗ P ∗ own γ (Excl ())) ∨ (Lock ↦ 1))%I.
+  Definition lock_inv (γ : gname) (i: addr) (P : iProp Σ) : iProp Σ :=
+    ((i ↦ 0 @N ∗ P ∗ own γ (Excl ())) ∨ (i ↦ 1 @N))%I.
 
-  Definition is_lock (N: namespace) (γ: gname) (P: iProp Σ) : iProp Σ :=
-    (inv N (lock_inv γ P))%I.
+  Definition is_lock (N: namespace) (γ: gname) (i: addr) (P: iProp Σ) : iProp Σ :=
+    (inv N (lock_inv γ i P))%I.
 
   Definition locked (γ: gname) : iProp Σ :=
     own γ (Excl ()).
 
-  Global Instance is_lock_persistent N γ R : Persistent (is_lock N γ R).
+  Global Instance is_lock_persistent N γ i R : Persistent (is_lock N γ i R).
   Proof. apply _. Qed.
 
   Global Instance locked_timless γ : Timeless (locked γ).
   Proof. apply _. Qed.
 
-  Lemma lock_init N (R: iProp Σ) E : Lock ↦ 0 -∗ R ={E}=∗ ∃ γ, is_lock N γ R.
+  Lemma lock_init N i (R: iProp Σ) E : i ↦ 0 @N -∗ R ={E}=∗ ∃ γ, is_lock N γ i R.
   Proof.
     iIntros "Hl HR".
     iMod (own_alloc (Excl ())) as (γ) "Hexcl"; first done.
-    iMod (inv_alloc N _ (lock_inv γ R) with "[-]").
+    iMod (inv_alloc N _ (lock_inv γ i R) with "[-]").
     { iNext. iLeft; iFrame. }
     iModIntro; iExists _; done.
   Qed.
 
-  Lemma wp_lock N γ (R: iProp Σ):
-    {{{ is_lock N γ R }}} lock {{{ RET tt; locked γ ∗ R }}}.
+  Lemma wp_lock N γ i (R: iProp Σ):
+    {{{ is_lock N γ i R }}} lock i {{{ RET tt; locked γ ∗ R }}}.
   Proof.
     iIntros (Φ) "#Hlock HΦ". iLöb as "IH".
     wp_loop; wp_bind.
@@ -230,14 +277,14 @@ Section lock.
       rewrite //=. wp_ret. iApply "IH"; eauto.
   Qed.
 
-  Lemma wp_unlock N γ (R: iProp Σ):
-    {{{ is_lock N γ R ∗ locked γ ∗ R }}} unlock {{{ RET tt; True }}}.
+  Lemma wp_unlock N γ i (R: iProp Σ):
+    {{{ is_lock N γ i R ∗ locked γ ∗ R }}} unlock i {{{ RET tt; True }}}.
   Proof.
     iIntros (Φ) "(#Hlock&Hlocked&HR) HΦ".
     iInv N as "[HL|>HUL]".
     - iDestruct "HL" as "(>H&?&>Htok)".
       iDestruct (own_valid_2 with "Htok Hlocked") as %H => //=.
-    - iApply (wp_write with "[$]"); iIntros "!> H !>".
+    - iApply (wp_write_mem with "[$]"); iIntros "!> H !>".
       iSplitR "HΦ"; last by iApply "HΦ".
       iLeft. iFrame.
   Qed.
