src/Examples/StatDb/Impl.v
@@ -1,65 +1,8 @@
 From Coq Require Import List.
 
 From RecoveryRefinement Require Export Lib.
+Require Import ExMach.ExMachAPI.
 
-Module Var.
-  Inductive id := Sum | Count | Lock.
-  Inductive Op : Type -> Type :=
-  | Read (i:id) : Op nat
-  | Write (i:id) (v:nat) : Op unit
-  | CAS (i:id) (vold: nat) (vnew:nat) : Op nat .
-  Definition State := (nat * nat * nat)%type.
-
-  Definition get (i:id) : State -> nat :=
-    match i with
-    | Sum => fun '(x, _, _) => x
-    | Count => fun '(_, y, _) => y
-    | Lock => fun '(_, _, z) => z
-    end.
-
-  Definition set (i:id) (v:nat) : State -> State :=
-    match i with
-    | Sum => fun '(_, y, z) => (v, y, z)
-    | Count => fun '(x, _, z) => (x, v, z)
-    | Lock => fun '(x, y, _) => (x, y, v)
-    end.
-
-  Import RelationNotations.
-  Definition cas_rel (i: id) (vold: nat) (vnew: nat): RelationAlgebra.relation State State nat :=
-    v <- reads (get i);
-    if nat_eq_dec v vold then
-        puts (set i vnew);;
-        pure v
-    else
-        pure v.
-
-  Definition dynamics : Dynamics Op State :=
-    {| step T (op: Op T) :=
-         match op with
-         | Read i => reads (get i)
-         | Write i v => puts (set i v)
-         | CAS i vold vnew => cas_rel i vold vnew
-         end;
-       crash_step :=
-         puts (fun _ => (0, 0, 0)); |}.
-
-  Lemma crash_total_ok (s: State):
-    exists s', dynamics.(crash_step) s (Val s' tt).
-  Proof. eexists; econstructor. Qed.
-
-  Lemma crash_non_err_ok (s: State) ret:
-    dynamics.(crash_step) s ret -> ret ≠ Err.
-  Proof. inversion 1; congruence. Qed.
-
-  Definition l : Layer Op :=
-    {| Layer.State := State;
-       sem := dynamics;
-       trace_proj := fun _ => nil;
-       crash_preserves_trace := fun _ _ _ => eq_refl;
-       crash_total := crash_total_ok;
-       crash_non_err := crash_non_err_ok;
-       initP := fun s => s = (0, 0, 0)|}.
-End Var.
 
 Module DB.
   Inductive Op : Type -> Type :=
@@ -94,31 +37,22 @@ Module DB.
        initP := fun s => s = nil |}.
 End DB.
 
-Definition read i := Call (Var.Read i).
-Definition write i v := Call (Var.Write i v).
-Definition cas i vold vnew := Call (Var.CAS i vold vnew).
-
-Definition lock : proc Var.Op unit :=
-  Loop (fun (_ : unit) =>
-          x <- Call (Var.CAS Var.Lock 0 1);
-          Ret (if nat_eq_dec x 0 then
-                  DoneWithOutcome tt
-                else
-                  ContinueOutcome tt)
-       )%proc tt.
-Definition unlock : proc Var.Op unit := Call (Var.Write Var.Lock 0).
+Definition sum_addr := 0.
+Definition count_addr := 1.
+Definition lock_addr := 2.
 
 Definition add n :=
-  (_ <- lock;
-   sum <- read Var.Sum; _ <- write Var.Sum (n + sum)%nat;
-   count <- read Var.Count; _ <- write Var.Count (1 + count)%nat;
-   unlock)%proc.
+  (_ <- lock lock_addr;
+   sum <- read_mem sum_addr; _ <- write_mem sum_addr (n + sum)%nat;
+   count <- read_mem count_addr; _ <- write_mem count_addr (1 + count)%nat;
+   unlock lock_addr)%proc.
 
 Definition avg :=
-  (_ <- lock;
-   sum <- read Var.Sum; count <- read Var.Count; _ <- unlock; Ret (sum/count)%nat)%proc.
+  (_ <- lock lock_addr;
+   sum <- read_mem sum_addr; count <- read_mem count_addr;
+   _ <- unlock lock_addr; Ret (sum/count)%nat)%proc.
 
-Definition impl : LayerImpl Var.Op DB.Op :=
+Definition impl : LayerImpl ExMach.Op DB.Op :=
   {| compile_op T (op: DB.Op T) :=
        match op with
        | DB.Add n => add n
