src/Examples/StatDb/Refinement.v
@@ -1,21 +1,23 @@
 From iris.algebra Require Import auth gmap.
 Require Export CSL.Refinement.
-Require Import StatDb.Impl StatDb.WeakestPre.
+Require Import StatDb.Impl ExMach.WeakestPre.
 Set Default Proof Using "Type".
 Unset Implicit Arguments.
 
 
 
 Section refinement_triples.
-  Context `{!varG Σ, !lockG Σ, !@cfgG (DB.Op) (DB.l) Σ}.
+  Context `{!exmachG Σ, !lockG Σ, !@cfgG (DB.Op) (DB.l) Σ}.
   Context (ρ : thread_pool DB.Op * DB.l.(State)).
 
-  Import Var.
+  Import ExMach.
 
   Definition DBLockInv :=
-    (∃ l, source_state l ∗ Sum ↦ (fold_right plus O l) ∗ Count ↦ (length l))%I.
+    (∃ l, source_state l
+          ∗ sum_addr ↦ (fold_right plus O l) @N
+          ∗ count_addr ↦ (length l) @N)%I.
 
-  Definition DBInv := (source_ctx ρ ∗ ∃ N γ, is_lock N γ DBLockInv)%I.
+  Definition DBInv := (source_ctx ρ ∗ ∃ N γ, is_lock N γ lock_addr DBLockInv)%I.
 
   (* TODO: write smart tactics for applying the wp_primitives *)
   Lemma add_refinement {T} j K `{LanguageCtx DB.Op unit T DB.l K} n:
@@ -26,10 +28,10 @@ Section refinement_triples.
     wp_bind. iApply (wp_lock with "[$]").
     iIntros "!> (Hlocked&HDB)".
     iDestruct "HDB" as (l) "(Hsource&Hsum&Hcount)".
-    wp_bind. iApply (wp_read with "Hsum"). iIntros "!> Hsum".
-    wp_bind. iApply (wp_write with "[$]"). iIntros "!> Hsum".
-    wp_bind. iApply (wp_read with "Hcount"). iIntros "!> Hcount".
-    wp_bind. iApply (wp_write with "[$]"). iIntros "!> Hcount".
+    wp_bind. iApply (wp_read_mem with "Hsum"). iIntros "!> Hsum".
+    wp_bind. iApply (wp_write_mem with "[$]"). iIntros "!> Hsum".
+    wp_bind. iApply (wp_read_mem with "Hcount"). iIntros "!> Hcount".
+    wp_bind. iApply (wp_write_mem with "[$]"). iIntros "!> Hcount".
     iMod (ghost_step_lifting with "Hj Hsource_inv Hsource") as "(Hj&Hsource&_)".
     { do 2 eexists; split; last by eauto. econstructor. }
     { set_solver+. }
@@ -48,8 +50,8 @@ Section refinement_triples.
     wp_bind. iApply (wp_lock with "[$]").
     iIntros "!> (Hlocked&HDB)".
     iDestruct "HDB" as (l) "(Hsource&Hsum&Hcount)".
-    wp_bind. iApply (wp_read with "Hsum"). iIntros "!> Hsum".
-    wp_bind. iApply (wp_read with "Hcount"). iIntros "!> Hcount".
+    wp_bind. iApply (wp_read_mem with "Hsum"). iIntros "!> Hsum".
+    wp_bind. iApply (wp_read_mem with "Hcount"). iIntros "!> Hcount".
     iMod (ghost_step_lifting with "Hj Hsource_inv Hsource") as "(Hj&Hsource&_)".
     { do 2 eexists; split; last by eauto. econstructor. }
     { set_solver+. }
