src/ShouldBuild.v
@@ -3,5 +3,5 @@
 From RecoveryRefinement Require Import Database.Store.
 From RecoveryRefinement Require Import CSL.RefinementAdequacy.
 From RecoveryRefinement Require Import CSL.Lifting.
-From RecoveryRefinement Require Import Examples.StatDb.WeakestPre.
+From RecoveryRefinement Require Import Examples.ExMach.WeakestPre.
 From RecoveryRefinement Require Import Examples.StatDb.Refinement.
